Minor additions to cv<->term transfer theorems

examples/algorithms/unification/triangular/first-order/cvtermScript.sml
@@ -17,30 +17,83 @@ Definition t2c_def:
   t2c cf (term$Const c) = cp (cn 2) (cf c)
 End
 
-Definition TmC_def:
+Definition TmC_def[simp]:
   (TmC AC (term$Var n) c ⇔ c = cp (cn 0) (cn n)) ∧
   (TmC AC (term$Pair t1 t2) c ⇔ ∃c1 c2. c = cp (cn 1) (cp c1 c2) ∧
                                         TmC AC t1 c1 ∧ TmC AC t2 c2) ∧
   (TmC AC (term$Const ct) c ⇔ ∃c0. c = cp (cn 2) c0 ∧ AC ct c0)
 End
 
+Theorem TmC_RIGHT_THM[simp]:
+  (TmC AC t (cp (cn 0) (cn n)) ⇔ t = Var n) ∧
+  (TmC AC t (cp (cn 1) (cp c1 c2)) ⇔
+     ∃t1 t2. t = Pair t1 t2 ∧ TmC AC t1 c1 ∧ TmC AC t2 c2) ∧
+  (TmC AC t (cp (cn 2) c) ⇔ ∃a. AC a c ∧ t = Const a)
+Proof
+  simp[EQ_IMP_THM, PULL_EXISTS] >> rpt conj_tac >>
+  Cases_on ‘t’ >> simp[]
+QED
+
 Theorem TmVar_C[transfer_rule]:
   (NC |==> TmC AC) term$Var (cp (cn 0))
 Proof
-  simp[FUN_REL_def, TmC_def, NC_def]
+  simp[FUN_REL_def, NC_def]
 QED
 
 Theorem TmPair_C[transfer_rule]:
   (TmC AC |==> TmC AC |==> TmC AC) term$Pair (λc1 c2. cp (cn 1) (cp c1 c2))
 Proof
-  simp[FUN_REL_def, TmC_def]
+  simp[FUN_REL_def]
 QED
 
 Theorem TmConst_C[transfer_rule]:
   (AC |==> TmC AC) term$Const (cp (cn 2))
 Proof
-  simp[FUN_REL_def, TmC_def]
+  simp[FUN_REL_def]
 QED
 
+Theorem total_TmC[transfer_simp]:
+  total AC ⇒ total (TmC AC)
+Proof
+  simp[total_def] >> strip_tac >> Induct >> gvs[] >> metis_tac[]
+QED
+
+Theorem left_unique_TmC[transfer_simp]:
+  left_unique AC ⇒ left_unique (TmC AC)
+Proof
+  simp[left_unique_def] >> strip_tac >> Induct >> gvs[PULL_EXISTS] >>
+  metis_tac[]
+QED
+
+Theorem right_unique_TmC[transfer_simp]:
+  right_unique AC ⇒ right_unique (TmC AC)
+Proof
+  simp[right_unique_def] >> strip_tac >> Induct >> gvs[PULL_EXISTS] >>
+  metis_tac[]
+QED
+
+Inductive is_cvterm:
+[~var:]
+  is_cvterm Cs (cp (cn 0) (cn n))
+[~pair:]
+  is_cvterm Cs c1 ∧ is_cvterm Cs c2 ⇒
+  is_cvterm Cs (cp (cn 1) (cp c1 c2))
+[~const:]
+  c ∈ Cs ⇒ is_cvterm Cs (cp (cn 2) c)
+End
+
+Theorem RRANGE_TmC[transfer_simp]:
+  RRANGE (TmC AC) = is_cvterm (RRANGE AC)
+Proof
+  simp[relationTheory.RRANGE, FUN_EQ_THM, EQ_IMP_THM, FORALL_AND_THM,
+       PULL_EXISTS] >> conj_tac >~
+  [‘TmC _ _ _ ⇒ _’]
+  >- (rpt gen_tac >> rename [‘TmC AC t c’] >> qid_spec_tac ‘c’ >>
+      Induct_on ‘t’ >> simp[is_cvterm_rules, PULL_EXISTS] >>
+      rw[] >> irule is_cvterm_const >>
+      simp[IN_DEF, relationTheory.RRANGE, SF SFY_ss]) >>
+  Induct_on ‘is_cvterm’ >> simp[IN_DEF, relationTheory.RRANGE] >>
+  metis_tac[]
+QED
 
 val _ = export_theory();
